bigodafny/solutions-unverified/1733/1733_49.dfy
@@ -52,31 +52,89 @@ function IndexOfInt(s: seq<int>, v: int): int
   else 1 + IndexOfInt(s[1..], v)
 }
 
+lemma IndexOfFindsLeftmost(s: seq<int>, v: int)
+  requires v in s
+  ensures 0 <= IndexOfInt(s, v) < |s|
+  ensures s[IndexOfInt(s, v)] == v
+  ensures forall t :: 0 <= t < IndexOfInt(s, v) ==> s[t] != v
+  decreases |s|
+{
+  if s[0] == v {
+  } else {
+    IndexOfFindsLeftmost(s[1..], v);
+  }
+}
+
+lemma ReverseIntElems(s: seq<int>)
+  ensures forall t :: 0 <= t < |s| ==> ReverseInt(s)[t] == s[|s| - 1 - t]
+  decreases |s|
+{
+  if |s| == 0 {
+  } else {
+    ReverseIntElems(s[1..]);
+  }
+}
+
+lemma ReverseIntMembership(s: seq<int>)
+  ensures forall v :: v in ReverseInt(s) <==> v in s
+  decreases |s|
+{
+  if |s| == 0 {
+  } else {
+    ReverseIntMembership(s[1..]);
+  }
+}
+
 method Solve(a: int, b_list: seq<int>) returns (output: string)
   requires |b_list| == a
+  requires forall v :: 1 <= v <= a ==> v in b_list
 {
   var n := a;
   var c: seq<int> := b_list;
   if n % 2 == 1 {
+    var cOld0 := c;
     var nc: seq<int> := [];
     var k := 0;
     while k < |c|
       invariant 0 <= k <= |c|
+      invariant |nc| == k
+      invariant forall t :: 0 <= t < k ==> nc[t] == n + 1 - cOld0[t]
       decreases |c| - k
     {
       nc := nc + [n + 1 - c[k]];
       k := k + 1;
     }
     c := nc;
+    assert forall v :: 1 <= v <= n ==> v in c by {
+      forall v | 1 <= v <= n
+        ensures v in c
+      {
+        assert 1 <= n + 1 - v <= n;
+        assert n + 1 - v in cOld0;
+        IndexOfFindsLeftmost(cOld0, n + 1 - v);
+        var idx := IndexOfInt(cOld0, n + 1 - v);
+        assert 0 <= idx < |cOld0| && cOld0[idx] == n + 1 - v;
+        assert c[idx] == n + 1 - cOld0[idx];
+        assert c[idx] == v;
+      }
+    }
   }
   var q := 0;
   var o: seq<string> := [];
   var i := 0;
   while i < n
     invariant 0 <= i <= n
+    invariant |c| == n
+    invariant forall t :: 0 <= t < i ==> c[t] == t + 1
+    invariant forall v :: 1 <= v <= n ==> v in c
     decreases n - i
   {
+    assert i + 1 in c by {
+      assert 1 <= i + 1 <= n;
+    }
+    IndexOfFindsLeftmost(c, i + 1);
     var j := IndexOfInt(c, i + 1);
+    assert i <= j;
     var m: seq<int> := RepeatInt(1, i);
     if j - i + 1 != 0 {
       m := m + [j - i + 1];
@@ -84,8 +142,32 @@ method Solve(a: int, b_list: seq<int>) returns (output: string)
     var tail := n - 1 - j;
     var tailN := if tail < 0 then 0 else tail;
     m := m + RepeatInt(1, tailN);
-    var mid := ReverseInt(c[i..j + 1]);
+    var seg := c[i..j + 1];
+    var mid := ReverseInt(seg);
+    ReverseIntElems(seg);
+    ReverseIntMembership(seg);
+    assert mid[0] == c[j];
+    var cOld := c;
     c := c[..i] + mid + c[j + 1..];
+    assert c[i] == i + 1 by {
+      assert (mid + cOld[j + 1..])[0] == mid[0];
+    }
+    assert forall t :: 0 <= t < i ==> c[t] == t + 1 by {
+      assert c[..i] == cOld[..i];
+    }
+    assert forall v :: 1 <= v <= n ==> v in c by {
+      forall v | 1 <= v <= n
+        ensures v in c
+      {
+        assert v in cOld;
+        assert cOld == cOld[..i] + seg + cOld[j + 1..];
+        if v in cOld[..i] {
+        } else if v in seg {
+          assert v in mid;
+        } else {
+        }
+      }
+    }
     if |m| > 1 {
       q := q + 1;
       if i % 2 == 1 {
