bigodafny/solutions-unverified/1861/1861_28.dfy
@@ -30,17 +30,25 @@ include "../../prelude.dfy"
 import opened Prelude
 
 method Solve(a: int, b: int, c: int) returns (output: string)
+  requires 1 <= b
+  requires 1 <= c <= b
 {
   var H := a; var W := b; var K := c;
   var MOD := 1000000007;
   var pats: seq<seq<int>> := [[0]];
   var i := 1;
   while i < W
+    invariant 1 <= i <= W
+    invariant forall t :: 0 <= t < |pats| ==> |pats[t]| == i
+    invariant forall t :: 0 <= t < |pats| ==> forall u :: 0 <= u < |pats[t]| ==> 0 <= pats[t][u] < i
     decreases W - i
   {
     var branch1: seq<seq<int>> := [];
     var j := 0;
     while j < |pats|
+      invariant 0 <= j <= |pats|
+      invariant forall t :: 0 <= t < |branch1| ==> |branch1[t]| == i + 1
+      invariant forall t :: 0 <= t < |branch1| ==> forall u :: 0 <= u < |branch1[t]| ==> 0 <= branch1[t][u] < i + 1
       decreases |pats| - j
     {
       branch1 := branch1 + [pats[j] + [i]];
@@ -49,6 +57,9 @@ method Solve(a: int, b: int, c: int) returns (output: string)
     var branch2: seq<seq<int>> := [];
     j := 0;
     while j < |pats|
+      invariant 0 <= j <= |pats|
+      invariant forall t :: 0 <= t < |branch2| ==> |branch2[t]| == i + 1
+      invariant forall t :: 0 <= t < |branch2| ==> forall u :: 0 <= u < |branch2[t]| ==> 0 <= branch2[t][u] < i + 1
       decreases |pats| - j
     {
       var p := pats[j];
@@ -63,16 +74,22 @@ method Solve(a: int, b: int, c: int) returns (output: string)
   var rs: seq<int> := seq(W, k requires 0 <= k < W => if k == 0 then 1 else 0);
   var row := 0;
   while row < H
+    invariant |rs| == W
+    invariant forall t :: 0 <= t < |pats| ==> |pats[t]| == W
+    invariant forall t :: 0 <= t < |pats| ==> forall u :: 0 <= u < |pats[t]| ==> 0 <= pats[t][u] < W
     decreases H - row
   {
     var newrs: seq<int> := [];
     var col := 0;
     while col < W
+      invariant 0 <= col <= W
+      invariant |newrs| == col
       decreases W - col
     {
       var s := 0;
       var pi := 0;
       while pi < |pats|
+        invariant 0 <= pi <= |pats|
         decreases |pats| - pi
       {
         s := (s + rs[pats[pi][col]]) % MOD;
