bigodafny/solutions-unverified/1871/1871_156.dfy
@@ -25,17 +25,59 @@
 include "../../prelude.dfy"
 import opened Prelude
 
+lemma GcdNonneg(a: int, b: int)
+  requires a >= 0 && b >= 0
+  ensures Gcd(a, b) >= 0
+  decreases b
+{
+  if b == 0 {
+  } else {
+    GcdNonneg(b, a % b);
+  }
+}
+
+lemma GcdPositive(a: int, b: int)
+  requires a >= 0 && b >= 0
+  requires a >= 1 || b >= 1
+  ensures Gcd(a, b) >= 1
+  decreases b
+{
+  if b == 0 {
+  } else {
+    GcdPositive(b, a % b);
+  }
+}
+
 method Solve(n: int, a_list: seq<int>) returns (output: string)
+  requires |a_list| >= 2
+  requires n <= |a_list|
+  requires forall v :: v in a_list ==> v >= 1
 {
   var lst := SortInts(a_list);
+  SortIntsKeepsElems(a_list);
+  assert {:split_here} forall v :: v in lst ==> v >= 1;
+  assert lst[0] in lst && lst[1] in lst;
+  assert lst[0] >= 1 && lst[1] >= 1;
   var g := Gcd(lst[0], lst[1]);
+  GcdPositive(lst[0], lst[1]);
+  assert {:split_here} g >= 1;
   var l := (lst[0] * lst[1]) / g;
+  assert {:split_here} l >= 0;
   var i := 2;
   while i < n
+    invariant 2 <= i
+    invariant g >= 1
+    invariant l >= 0
     decreases n - i
   {
+    assert {:split_here} lst[i] in lst;
+    assert lst[i] >= 1;
     var gi := Gcd(g, lst[i]);
+    GcdPositive(g, lst[i]);
+    assert {:split_here} gi >= 1;
     var running := (lst[i] * g) / gi;
+    assert {:split_here} running >= 0;
+    GcdNonneg(l, running);
     l := Gcd(l, running);
     g := Gcd(g, lst[i]);
     i := i + 1;
