bigodafny/solutions-unverified/1871/1871_291.dfy
@@ -28,17 +28,57 @@
 include "../../prelude.dfy"
 import opened Prelude
 
+lemma GcdNonneg(a: int, b: int)
+  requires a >= 0 && b >= 0
+  ensures Gcd(a, b) >= 0
+  decreases b
+{
+  if b == 0 {
+  } else {
+    GcdNonneg(b, a % b);
+  }
+}
+
+lemma GcdPositive(a: int, b: int)
+  requires a >= 0 && b >= 0
+  requires a >= 1 || b >= 1
+  ensures Gcd(a, b) >= 1
+  decreases b
+{
+  if b == 0 {
+  } else {
+    GcdPositive(b, a % b);
+  }
+}
+
 method Solve(n: int, a_list: seq<int>) returns (output: string)
+  requires |a_list| >= 2
+  requires forall v :: v in a_list ==> v >= 1
 {
   var arr := a_list;
+  assert arr[0] in arr && arr[1] in arr;
+  assert {:split_here} arr[0] >= 1 && arr[1] >= 1;
+  GcdPositive(arr[0], arr[1]);
   var lcm := (arr[0] * arr[1]) / Gcd(arr[0], arr[1]);
+  assert {:split_here} lcm >= 0;
   var current := lcm;
   var i := 2;
   while i < |arr|
+    invariant 2 <= i
+    invariant current >= 0
+    invariant lcm >= 0
     decreases |arr| - i
   {
-    var running := (current * arr[i]) / Gcd(current, arr[i]);
+    assert {:split_here} arr[i] in arr;
+    assert arr[i] >= 1;
+    GcdPositive(current, arr[i]);
+    var gi := Gcd(current, arr[i]);
+    assert {:split_here} gi >= 1;
+    var running := (current * arr[i]) / gi;
+    assert {:split_here} running >= 0;
+    GcdNonneg(lcm, running);
     lcm := Gcd(lcm, running);
+    GcdNonneg(current, arr[i]);
     current := Gcd(current, arr[i]);
     i := i + 1;
   }
